trunk/meta/Unbound_results.v
@@ -1,0 +1,109 @@
+Add LoadPath "metatheory".
+Require Import Coq.Arith.Wf_nat.
+Require Import Coq.Logic.FunctionalExtensionality.
+Require Import Coq.Program.Equality.
+
+Require Export Metatheory.
+Require Export LibLNgen.
+
+Require Export Unbound.
+
+Set Implicit Arguments.
+
+
+
+Lemma beq_nat_sym : forall n1 n2 b, beq_nat n1 n2 = b -> beq_nat n2 n1 = b.
+induction n1; destruct n2; simpl; auto.
+Qed.
+
+Lemma case_bool : forall b:bool, {b = true} + {b = false}.
+intro b. destruct b. auto. auto.
+Qed.
+
+Lemma aeq_sym : forall t u m, aeq m t u = true -> aeq m u t = true.
+induction t; intros u m; destruct m; destruct u; simpl in *; 
+   try (intro H; 
+        destruct (andb_prop _ _ H);
+        rewrite (IHt1 _ _); auto;
+        rewrite (IHt2 _ _); auto);
+auto using beq_nat_sym.
+destruct (case_bool (beq_nat n n1)).
+rewrite e.
+rewrite (beq_nat_sym n n1 e). 
+auto using beq_nat_sym.
+rewrite e. 
+rewrite (beq_nat_sym n n1 e). auto.
+destruct (case_bool (beq_nat n n1));
+  rewrite e; rewrite (beq_nat_sym n n1 e); auto using beq_nat_sym.
+destruct (n == n0); destruct (n0 == n); auto.
+Qed.
+
+Lemma beq_nat_trans : forall n1 n2 n3, beq_nat n1 n2 = true ->
+  beq_nat n2 n3 = true -> beq_nat n1 n3 = true.
+induction n1; destruct n2;
+induction n3; simpl; auto. intros. inversion H.
+apply IHn1.
+Qed.
+
+Lemma aeq_trans : forall s t u m, aeq m s t = true -> aeq m t u = true -> aeq m s u = true.
+induction s; destruct t; destruct u; intro m; simpl; try (intro H; inversion H); auto.
+Admitted.
+
+Lemma aeq_fv : forall t1 t2 m, aeq m t1 t2 = true -> fv m t1 = fv m t2.
+induction t1; destruct t2; intro m; simpl; try (intro H; inversion H); auto.
+destruct m; simpl in *; 
+  auto;
+  try (destruct (andb_prop _ _ H);
+      rewrite (IHt1_1 t2_1); auto;
+      rewrite (IHt1_2 t2_2); auto);
+  auto.
+destruct (n == n0). subst. auto. inversion H.
+destruct (andb_prop _ _ H).
+rewrite (IHt1_1 t2_1); auto.
+rewrite (IHt1_2 t2_2); auto.
+destruct (andb_prop _ _ H).
+rewrite (IHt1_1 t2_1); auto.
+rewrite (IHt1_2 t2_2); auto. 
+destruct (andb_prop _ _ H).
+rewrite (IHt1_1 t2_1); auto.
+rewrite (IHt1_2 t2_2); auto. 
+Qed. 
+
+Lemma aeq_subst : forall t1 t2 s1 s2 x m, 
+  aeq m t1 t2 = true -> aeq Term s1 s2 = true -> 
+  aeq m (subst m s1 x t1) (subst m s2 x t2) = true.
+induction t1; destruct t2; intros s1 s2 x m; try (intro H; inversion H);
+  try (destruct (andb_prop _ _ H1);
+    rewrite H0; rewrite H2; simpl;
+    intro J; rewrite IHt1_1; auto; rewrite IHt1_2; auto); auto.
+
+destruct m.
+  simpl. destruct (n == n0). subst. destruct (n0 == x). auto. auto.
+    inversion H1.
+  simpl. auto.
+rewrite H1. intro J. simpl. rewrite IHt1; auto.
+rewrite H1. intro J. simpl. rewrite IHt1; auto.
+rewrite H1. intro J. simpl. rewrite IHt1; auto.
+Qed.
+
+Lemma aeq_freshen_pat : forall pat pat1 pat2 ns1 ns1' ns2 ns2' perm1 perm2,
+  freshen pat1 ns1 nil = (pat, ns1', perm1) ->
+  freshen pat2 ns2 nil = (pat, ns2', perm2) ->
+  aeq Pat pat1 pat2 = true.
+induction pat; destruct pat1; simpl; 
+   intros pat2' ns1 ns1' ns2 ns2' perm1 perm2 J1 J2; try inversion J1; subst.
+destruct pat2'; simpl in *; inversion J2. subst.
+rewrite <- beq_nat_refl.
+rewrite <- beq_nat_refl. auto.
+destruct ns2;  inversion J2.
+
+Lemma aeq_freshen : forall t1 t2 pat pat1 pat2 ns1 ns1' ns2 ns2' perm1 perm2,
+  freshen Pat pat1 ns1 nil = (pat, ns1', perm1) ->
+  freshen Pat pat2 ns2 nil = (pat, ns2', perm2) ->
+  aeq Term (swaps perm1 t1) (swaps perm2 t2) = true ->
+  aeq Term (bind pat1 t1) (bind pat2 t2) = true.
+induction t1; destruct t2; simpl;
+  intros pat pat1 pat2 ns1 ns1' ns2 ns2' perm1 perm2 H1 H2 H3;
+  try inversion H3.
+(* 1 *)
+rewrite H3. 
